Test/AbsHoudini/test1.bpl
@@ -2,7 +2,7 @@ var g: bool;
 
 procedure foo() 
 modifies g;
-ensures b0 ==> (!old(g) ==> old(g) == g);
+ensures b0() || (!old(g) ==> old(g) == g);
 {
   call AcquireLock();
   call ReleaseLock();
@@ -10,14 +10,14 @@ ensures b0 ==> (!old(g) ==> old(g) == g);
 
 procedure AcquireLock()
 modifies g;
-ensures b1 ==> old(g) == g;
+ensures b1() || old(g) == g;
 {
   g := true;
 }
 
 procedure ReleaseLock()
 modifies g;
-ensures b2 ==> old(g) == g;
+ensures b2() || old(g) == g;
 {
   g := false;
 }
@@ -27,10 +27,12 @@ modifies g;
 {
   g := false;
   call foo();
-  assert !g;
+  assert Assert() || !g;
 }
 
-const {:existential true} b0: bool;
-const {:existential true} b1: bool;
-const {:existential true } b2: bool;
+function {:existential true} b0(): bool;
+function {:existential true} b1(): bool;
+function {:existential true } b2(): bool;
+function {:existential true} Assert(): bool;
 
+// Expected: b0 = false, b1 = true, b2 = true, Assert = false
