Test/AbsHoudini/test10.bpl
@@ -1,9 +1,9 @@
 var sdv_7: int;
 var sdv_21: int;
-const {:existential true} b1: bool;
-const{:existential true}  b2: bool;
-const{:existential true}  b3: bool;
-const{:existential true}  b4: bool;
+function {:existential true} b1(): bool;
+function{:existential true}  b2(): bool;
+function{:existential true}  b3(): bool;
+function{:existential true}  b4(): bool;
 
 procedure push(a:int)
 modifies sdv_7, sdv_21;
@@ -21,8 +21,8 @@ modifies sdv_7, sdv_21;
 
 procedure foo()
 modifies sdv_7, sdv_21;
-requires {:candidate} b1 ==> (sdv_7 == 0);
-ensures{:candidate}  b2 ==> (sdv_7 == old(sdv_7));
+requires {:candidate} b1() || (sdv_7 == 0);
+ensures{:candidate}  b2() || (sdv_7 == old(sdv_7));
 {
    call push(2);
    call pop();
@@ -30,8 +30,8 @@ ensures{:candidate}  b2 ==> (sdv_7 == old(sdv_7));
 }
 
 procedure bar()
-requires{:candidate} b3 ==> (sdv_7 == 0);
-ensures{:candidate}  b4 ==> (sdv_7 == old(sdv_7));
+requires{:candidate} b3() || (sdv_7 == 0);
+ensures{:candidate}  b4() || (sdv_7 == old(sdv_7));
 modifies sdv_7, sdv_21;
 {
    call push(1);
@@ -44,4 +44,7 @@ modifies sdv_7, sdv_21;
    sdv_7 := 0;
    call foo();
 }
+
+// Expected: All false
+
 
