Test/AbsHoudini/test7.bpl
@@ -1,3 +1,5 @@
+function {:existential true} Assert() : bool;
+
 var g: int;
 
 procedure main() 
@@ -5,7 +7,7 @@ modifies g;
 {
   g := 0;
   call foo();
-  assert g == 1;
+  assert Assert() || g == 1;
 }
 
 procedure foo() 
@@ -13,3 +15,5 @@ modifies g;
 {
   g := g + 1;
 }
+
+// Expected: Assert = false
