Test/AbsHoudini/test8.bpl
@@ -1,3 +1,5 @@
+function {:existential true} Assert(): bool;
+
 var g: int;
 
 procedure main() 
@@ -5,7 +7,7 @@ modifies g;
 {
   g := 0;
   call foo();
-  assert g == 1;
+  assert Assert() || g == 1;
 }
 
 procedure {:inline 1} foo() 
@@ -19,3 +21,5 @@ modifies g;
 {
   g := g + 1;
 }
+
+// Expected: Assert = false
